\documentclass{article}

% Document extensibility %
%
% Disables native paragraph indentation
\usepackage{parskip} 
%
% Provides further bullet options for lists
\usepackage{enumitem}

% Mathematical symbol and statement packages %
%
% Necessary
\usepackage{amsmath}
\usepackage{amssymb}
%
% Extensive fraction notation
\usepackage{xfrac}
%
% Generic mathematical commands
% Notable: \degree, \celcius
\usepackage{gensymb}
%
% Variable vector notation (arrow above variable)
\usepackage{esvect}
%
% Multiline boxed equations
\usepackage{empheq}
%
% SI Unit
\usepackage{siunitx}

% Graphic packages %
%
% Diagrams and illustrations
\usepackage{tikz}
%
% Image insertion
\usepackage{graphicx}

% Document content %
%
% Change title of table of contents
% \renewcommand{\contentsname}{Title}

\title{Week 03 Participation Assignment (2 of 3)}
\date{03 March 2023}
\author{Corey Mostero}

\begin{document}

% Command `\hr` to insert horizontal rules
\newcommand{\hr}{\par\noindent\rule{\textwidth}{0.4pt}}

\maketitle
\newpage

\tableofcontents

\section{Part 2}
Identify the equation as homogeneous, Bernoulli, or of the form $ y' = G(ax + by + c) $

\subsection{a)}
$$ 2xydx + (y^2 - x^2)dy = 0 $$
\begin{align*}
	(y^2 - x^2)dy & = -2xydx \\
	\frac{dy}{dx} & = \frac{-2xy}{y^2 - x^2} \\
				  & = \frac{-2xy}{x^2(\frac{y^2}{x^2} - 1)} \\
				  & = \frac{-2y}{x(\frac{y^2}{x^2} - 1)}
\end{align*}
\begin{equation*}
	\boxed{\text{homogeneous}}
\end{equation*}

\subsection{b)}
$$ (y - 4x - 1)^2dx - dy = 0 $$
\begin{align*}
	dy & = (y - 4x - 1)^2dx \\
	\frac{dy}{dx} & = (y - 4x - 1)^2
\end{align*}
\begin{equation*}
	\boxed{
		y' = G(ax + by + c)
	}
\end{equation*}

\subsection{c)}
$$ \frac{dy}{dx} + \frac{y}{x} - x^3y^2 = 0 $$
\begin{align*}
	\frac{dy}{dx} + \left( \frac{1}{x} \right)y & = (x^3)y^2
\end{align*}
\begin{equation*}
	\boxed{\text{Bernoulli}}
\end{equation*}

\subsection{d)}
$$ xdy - ydx = \sqrt{xy}dx $$
\begin{align*}
	(x)dy & = \sqrt{xy}dx + (y)dx \\
	(x)dy & = dx \left( \sqrt{xy} + y \right) \\
	\frac{dy}{dx} & = \frac{\left( \sqrt{xy} + y \right)}{x} \\
				  & = \frac{\sqrt{xy}}{x} + \frac{y}{x} \\
				  & = \frac{\sqrt{x^2(\frac{y}{x})}}{x} + \frac{y}{x} \\
				  & = \frac{x\sqrt{\frac{y}{x}}}{x} + \frac{y}{x} \\
				  & = \sqrt{\frac{y}{x}} + \frac{y}{x}
\end{align*}
\begin{equation*}
	\boxed{\text{homogeneous}}
\end{equation*}
\begin{align*}
	(x)\frac{dy}{dx} - y & = \sqrt{xy} \\
	\frac{dy}{dx} - \left( \frac{1}{x} \right) y & = \frac{\sqrt{xy}}{x} \\
	\frac{dy}{dx} - \left( \frac{1}{x} \right) y & = \left( \frac{\sqrt{x}}{x} \right) y^{\sfrac{1}{2}}
\end{align*}
\begin{equation*}
	\boxed{\text{Bernoulli}}
\end{equation*}

\subsection{e)}
$$ \frac{dy}{dx} = \sqrt{x + y} - 1 $$
\begin{align*}
	\frac{dy}{dx} & = \sqrt{x(1 + \frac{y}{x})} - 1
\end{align*}
\begin{equation*}
	\boxed{\text{homogeneous}}
\end{equation*}

\subsection{f)}
$$ \left( ye^{-2x} + y^3 \right)dx - e^{-2x}dy = 0 $$
\begin{align*}
	\left( e^{-2x} \right)dy & = \left( ye^{-2x} + y^3 \right)dx \\
	\frac{dy}{dx} & = \frac{ye^{-2x} + y^3}{e^{-2x}} \\
				  & = \frac{ye^{-2x}}{e^{-2x}} + \frac{y^3}{e^{-2x}} \\
				  & = y + \frac{y^3}{e^{-2x}} \\
	\frac{dy}{dx} - y & = \left( \frac{1}{e^{-2x}} \right) y^3
\end{align*}
\begin{equation*}
	\boxed{\text{Bernoulli}}
\end{equation*}

\end{document}
