\documentclass{article}

% Document extensibility %
%
% Disables native paragraph indentation
\usepackage{parskip} 
%
% Provides further bullet options for lists
\usepackage{enumitem}

% Mathematical symbol and statement packages %
%
% Necessary
\usepackage{amsmath}
\usepackage{amssymb}
%
% Extensive fraction notation
\usepackage{xfrac}
%
% Generic mathematical commands
% Notable: \degree, \celcius
\usepackage{gensymb}
%
% Variable vector notation (arrow above variable)
\usepackage{esvect}
%
% Multiline boxed equations
\usepackage{empheq}
%
% SI Unit
\usepackage{siunitx}

% Graphic packages %
%
% Diagrams and illustrations
\usepackage{tikz}
%
% Image insertion
\usepackage{graphicx}

% Document content %
%
% Change title of table of contents
% \renewcommand{\contentsname}{Title}

\begin{document}

% Command `\hr` to insert horizontal rules
\newcommand{\hr}{\par\noindent\rule{\textwidth}{0.4pt}}

% Command to box and center math equations
\newcommand{\bc}[1]{
	\begin{equation*}
		\begin{boxed}
			{#1}
		\end{boxed}
	\end{equation*}
}

% Command for single line equations with a condition
\newcommand{\cond}[2]{
	\ifmmode
		{#1} \quad {#2}
	\else
		$$ {#1} \quad {#2} $$
	\fi
}

\newcommand{\iu}{\mathrm{i}\mkern1mu}

\tableofcontents

\section{Section 5.3}

\subsection{5.3.1}
Find the general solution of the differential equation.
$$ y'' - 289y = 0 $$
\begin{align*}
	r^2 - 289 & = 0 \\
	r & = 17, -17 \\
	y(x) & = c_1e^{17x} + c_2^{-17x}
\end{align*}

\subsection{5.3.3}
Find the general solution of the differential equation.
$$ y'' + y' - 56y = 0 $$
\begin{align*}
	r^2 + r - 56 & = 0 \\
	r & = 7, -8 \\
	y(t) & = c_1e^{7t} + c_2e^{-8t}
\end{align*}

\subsection{5.3.4}
Find a general solution.
$$ 4y'' + 7y' - 2y = 0 $$
\begin{align*}
	4r^2 + 7r - 2 & = 0 \\
	r & = \frac{1}{4}, -2 \\
	y(t) & = c_1e^{\sfrac{t}{4}} + c_2e^{-2t}
\end{align*}

\subsection{5.3.5}
Find a general solution to the given differential equation.
$$ 4w'' + 12w' + 9w = 0 $$
\begin{align*}
	4r^2 + 12r + 9 & = 0 \\
	r & = -\frac{3}{2} \\
	w(t) & = c_1e^{-\sfrac{3t}{2}} + c_2te^{-\sfrac{3t}{2}}
\end{align*}

\subsection{5.3.7}
Find the general solution of the differential equation.
$$ 36y'' - 84y' + 49y = 0 $$
\begin{align*}
	36r^2 - 84r + 49 & = 0 \\
	r & = \frac{7}{6} \\
	y(x) & = c_1e^{\sfrac{7x}{6}} + xc_2e^{\sfrac{7x}{6}}
\end{align*}

\subsection{5.3.9}
The auxiliary equation for the given differential equation has complex roots. Find a general solution.
$$ y'' - 10y' + 29y = 0 $$
\begin{align*}
	r^2 - 10r + 29 & = 0 \\
	r & = 5 \pm 2\iu \\
	y(t) & = c_1e^{5t}\cos(2t) + c_2e^{5t}\sin(2t)
\end{align*}

\subsection{5.3.11}
Find the general solution of the differential equation.
$$ y^{(4)} - 32y^{(3)} + 256y'' = 0 $$
\begin{align*}
	r^4 - 32r^3 + 256r^2 & = 0 \\
	r & = 0, 0, 16, 16 \\
	y(x) & = c_1 + c_2x + c_3e^{16x} + c_4xe^{16x}
\end{align*}

\subsection{5.3.13}
Find the general solution of the differential equation.
$$ 9y^{(3)} + 12y'' + 4y' = 0 $$
\begin{align*}
	9r^3 + 12r^2 + 4r & = 0 \\
	r & = 0, -\frac{2}{3}, -\frac{2}{3} \\
	y(x) & = c_1 + c_2e^{-\sfrac{2x}{3}} + c_3xe^{-\sfrac{2x}{3}}
\end{align*}

\subsection{5.3.18}
Find the general solution of the differential equation.
$$ 256y^{(4)} = y $$
\begin{align*}
	256y^{(4)} - y & = 0 \\
	256r^4 - 1 & = 0 \\
	r & = 0 \pm \frac{1}{4}, 0 \pm \frac{1}{4}i \\
	y(x) & = c_1e^{\frac{x}{4}} + c_2e^{-\frac{x}{4}} + c_3\cos \left( \frac{x}{4} \right) + c_4\sin \left( \frac{x}{4} \right)
\end{align*}

\subsection{5.3.19}
Find three linearly independent solutions of the given third-order differential equation and write a general solution as an arbitrary linear combination of them.
$$ z''' + 7z'' - 5z' - 75z = 0 $$
\begin{align*}
	r^3 + 7r^2 - 5r - 75 & = 0 \\
	r & = -5, -5, 3 \\
	z(t) & = c_1e^{-5t} + c_2te^{-5t} + c_3e^{3t}
\end{align*}

\subsection{5.3.21}
Find the unique solution of the second-order initial value problem.
$$ y'' + 2y' - 15y = 0, y(0) = -1, y'(0) = -11 $$
\begin{align*}
	r^2 + 2r - 15 & = 0 \\
	r & = -5, 3 \\
	y(x) & = c_1e^{-5x} + c_2e^{3x} \\
	y'(x) & = -5c_1e^{-5x} + 3c_2e^{3x} \\
	y''(x) & = 25c_1e^{-5x} + 9c_2e^{3x}
\end{align*}
\begin{align*}
	y(0) & = c_1e^{-5(0)} + c_2e^{3(0)} = -1 \\
	c_1 + c_2 & = -1 \\
	c_1 & = -1 - c_2 \\
	y'(0) & = -5c_1e^{-5(0)} + 3c_2e^{3(0)} = -11 \\
	-5c_1 + 3c_2 & = -11 \\
	-5( -1 - c_2 ) + 3c_2 & = -11 \\
	c_2 & = -2 \\
	c_1 & = -1 - (-2) \\
	c_1 & = 1 \\
	y(x) & = e^{-5x} + -2e^{3x}
\end{align*}
\bc{y(x) = e^{-5x} + -2e^{3x}}

\subsection{5.3.23}
Solve the given initial value problem.
$$ y'' + 4y' + 29y = 0; y(0) = 3, y'(0) = -3 $$
\begin{align*}
	r^2 + 4r + 29 & = 0 \\
	r & = -2 \pm 5i \\
	y(t) & = c_1e^{-2t}\cos(5t) + c_2e^{-2t}\sin(5t)
\end{align*}
\begin{align*}
	y(t) & = c_1e^{-2t}\cos(5t) + c_2e^{-2t}\sin(5t) \\
	y(0) & = c_1e^{-2(0)}\cos(5(0)) + c_2e^{-2t(0)}\sin(5(0)) = 3 \\
	c_1 & = 3 \\
	y'(t) & = c_1(-e^{-2t}(5\sin(5t) + 2\cos(5t))) + c_2(-e^{-2t}(2\sin(5t) - 5\cos(5t))) \\
	y'(0) & = c_1(-e^{2(0)}(5\sin(5(0)) + 2\cos(5(0)))) + c_2(-e^{-2(0)}(2\sin(5(0)) - 5\cos(5(0)))) = -3 \\
	-2c_1 + 5c_2 & = -3 \\
	-2(3) + 5c_2 & = -3 \\
	c_2 & = \frac{3}{5} \\
	y(t) & = 3e^{-2t}\cos(5t) + \frac{3}{5}e^{-2t}\sin(5t)
\end{align*}
\bc{y(t) = 3e^{-2t}\cos(5t) + \frac{3}{5}e^{-2t}\sin(5t)}

\subsection{5.3.39}
Find a linear homogeneous constant-coefficient equation with the given general solution.
$$ (A + Bx + Cx^2 + Dx^3)e^{4x} $$
\bc{y^{(4)} - 16y^{(3)} + 96y'' - 256y' + 256y = 0}

\subsection{5.3.54}
A third-order Euler equation is one of the form $ ax^3y''' + bx^2y'' + cxy' + ky = 0 $, where $ a $, $ b $, $ c $, and $ k $ are constants. If $ x > 0 $, then the substitution $ v = \ln(x) $ transforms the equation into the constant coefficient linear equation below, with independent variable $ v $.
$$ a \frac{d^3y}{dv^3} + (b - 3a) \frac{d^2y}{dv^2} + (c - b + 2a)\frac{dy}{dv} + ky = 0 $$
Make the substitution $ v = \ln(x) $ to find the general solution of $ 2x^3y''' + 12x^2y'' + 8xy' = 0 $ for $ x > 0 $.
\begin{align*}
	2y''' + (12- 3(2))y'' + (8 - 12 + 2(2))y' & = 0 \\
	2y''' + 6y'' & = 0 \\
	2r^3 + 6y^2 & = 0 \\
	r & = 0, 0, -3 \\
	y(v) & = c_1 + c_2v + c_3e^{-3v} \\
	y(x) & = c_1 + c_2\ln(x) + \frac{c_3}{x^3}
\end{align*}

\end{document}
