\documentclass{article}

% Document extensibility %
%
% Disables native paragraph indentation
\usepackage{parskip} 
%
% Provides further bullet options for lists
% \usepackage{enumitem}
%
% 

% Mathematical symbol and statement packages %
%
% Necessary
\usepackage{amsmath}
\usepackage{amssymb}
%
% Extensive fraction notation
\usepackage{xfrac}
%
% Generic mathematical commands
% Notable: \degree, \celcius
\usepackage{gensymb}
%
% Variable vector notation (arrow above variable)
% \usepackage{esvect}

% Graphic packages %
%
% Diagrams and illustrations
% \usepackage{tikz}
%
% Image insertion
% \usepackage{graphicx}

% Document content %
%
% Change title of table of contents
% \renewcommand{\contentsname}{Title}

\usepackage{empheq}

\title{Week 01 and Week 02 Participation Assignment (3 of 4)}
\date{24 February 2023}
\author{Corey Mostero}

\begin{document}

% Command `\hr` to insert horizontal rules
\newcommand{\hr}{\par\noindent\rule{\textwidth}{0.4pt}}

\maketitle
\newpage

\tableofcontents

\section{Part 3}

\textbf{Directions:} We say a differential equation is separable if we can write the equation into the form of $ \frac{dy}{dx} = f(x) \cdot g(y) $. For the following differential equation, determine whether the given equation is separable or not. If it is separable, identify $ f $ and $ g $ (we may encounter other variables other than $ x $ and $ y $).  

\subsection{Problem 1}
$$ \frac{dy}{dx} - \sin(x + y) = 0 $$
\begin{align*}
    \frac{dy}{dx} - \sin(x + y) & = 0 \\
    \frac{dy}{dx} & = \sin(x + y) \\
    \frac{dy}{dx} & = \sin(x)\cos(y) + \cos(x)\sin(y)
\end{align*}
\begin{equation*}
    \boxed{\text{Cannot be turned into separable form.}}
\end{equation*}

\subsection{Problem 2}
$$ \frac{dy}{dx} = 4y^2 - 3y + 1 $$
\begin{align*}
    \frac{dy}{dx} & = 4y^2 - 3y + 1 \\
    \left(\frac{dx}{4y^2 -3y + 1}\right) \frac{dy}{dx} & = \left(4y^2 - 3y + 1\right) \left(\frac{dx}{4y^2 -3y + 1}\right) \\
    \left(\frac{1}{4y^2 -3y + 1}\right)dy & = (1)dx
\end{align*}
\begin{empheq}[box=\fbox]{align*}
    & \text{The differential equation is separable.} \\
    & f(x) = 1 \text{, } g(y) = 4y^2 - 3y + 1
\end{empheq}

\subsection{Problem 3}
$$ \frac{ds}{dt} = t\ln \left(s^{2t}\right) + 8t^2 $$
\begin{align*}
    \frac{ds}{dt} & = t\ln \left(s^{2t}\right) + 8t^2 \\
                  & = t(2t)\ln(s) + 8t^2 \\
                  & = 2t^2\ln(s) + 8t^2 \\
                  & = (2t^2)(\ln(s) + 4) \\
    \left(\frac{1}{\ln(s)+4}\right)ds & = (2t^2)dt
\end{align*}
\begin{empheq}[box=\fbox]{align*}
    & \text{The differential equation is separable.} \\
    & f(s) = \ln(s) + 4 \text{, } g(t) = 2t^2
\end{empheq}

\subsection{Problem 4}
$$ \frac{dy}{dx} = \frac{ye^{x+y}}{x^2+2} $$
\begin{align*}
    \frac{dy}{dx} & = \frac{ye^{x+y}}{x^2+2} \\
                  & = \frac{ye^xe^y}{x^2+2} \\
    \frac{dy}{dx} & = \left(ye^y\right) \left(\frac{e^x}{x^2+2}\right)
\end{align*}
\begin{empheq}[box=\fbox]{align*}
    & \text{The differential equation is separable.} \\
    & f(x) = \left(\frac{e^x}{x^2+2}\right) \text{, } g(y) = ye^y
\end{empheq}

\subsection{Problem 5}
$$ \left(xy^2 + 3y^2\right)dy - 2xdx = 0 $$
\begin{align*}
    \left(xy^2 + 3y^2\right)dy - 2xdx & = 0 \\
    \left(xy^2 + 3y^2\right)dy & = (2x)dx \\
    \frac{dy}{dx}\left(xy^2 + 3y^2\right) & = 2x \\
    \frac{dy}{dx} & = \frac{2x}{xy^2 + 3y^2} \\
                  & = \frac{2x}{y^2\left(x + 3\right)} \\
    \frac{dy}{dx} & = \left(\frac{1}{y^2}\right) \left(\frac{2x}{x+3}\right)
\end{align*}
\begin{empheq}[box=\fbox]{align*}
    & \text{The differential equation is separable.} \\
    & f(x) = \left(\frac{2x}{x+3}\right) \text{, } g(y) = \left(\frac{1}{y^2}\right)
\end{empheq}

\subsection{Problem 6}
$$ s^2 + \frac{ds}{dt} = \frac{s+1}{st} $$
\begin{align*}
    s^2 + \frac{ds}{dt} & = \frac{s+1}{st} \\
    \frac{ds}{dt} & = \frac{s+1}{st} - s^2 \\
                  & = \frac{s}{st} + \frac{1}{st} - s^2 \\
                  & = \frac{1}{t} + \frac{1}{st} - s^2 \\
                  & = \frac{1}{t}\left(1 + \frac{1}{s}\right) - s^2
\end{align*}
\begin{equation*}
    \boxed{\text{Cannot be turned into separable form.}}
\end{equation*}

\end{document}
