\documentclass{article}

% Document extensibility %
%
% Disables native paragraph indentation
\usepackage{parskip} 
%
% Provides further bullet options for lists
\usepackage{enumitem}

% Mathematical symbol and statement packages %
%
% Necessary
\usepackage{amsmath}
\usepackage{amssymb}
%
% Extensive fraction notation
\usepackage{xfrac}
%
% Generic mathematical commands
% Notable: \degree, \celcius
\usepackage{gensymb}
%
% Variable vector notation (arrow above variable)
\usepackage{esvect}
%
% Multiline boxed equations
\usepackage{empheq}

% Graphic packages %
%
% Diagrams and illustrations
\usepackage{tikz}
%
% Image insertion
\usepackage{graphicx}

% Document content %
%
% Change title of table of contents
\renewcommand{\contentsname}{Homework: Section 1.5}

\begin{document}

% Command `\hr` to insert horizontal rules
\newcommand{\hr}{\par\noindent\rule{\textwidth}{0.4pt}}

\tableofcontents
\newpage

\section{Practice Problems}

\subsection{Problem 1}

Find the general solution of the differential equation. Then, use the initial condition to find the corresponding particular solution.
$$ \frac{dy}{dx} - 4y = 6e^{4x} \text{, } y(0) = 0 $$
\begin{align*}
    \frac{dy}{dx} - 4y & = 6e^{4x} \text{ already separated} \\
                       & \therefore P(x) = -4, \rho(x) = e^{\int(-4)dx} \\
    y(x) & = e^{\int(4)dx} \left[ \int \left( 6e^{4x}e^{\int(-4)dx} \right) dx + C \right] \\
         & = e^{4x} \int \left( 6e^{4x}e^{-4x} \right)dx + Ce^{4x} \\
         & = e^{4x} \int (6)dx + Ce^{4x} \\
    y(0) & = e^{4(0)} (6(0)) + Ce^{4(0)} = 0 \\
    C & = 0 \\
\end{align*}
\begin{equation*}
    \boxed{
        y(x) = \frac{6x}{e^{-4x}} + Ce^{4x}, y(0) \rightarrow y(x) = \frac{6x}{e^{-4x}}
    }
\end{equation*}

\subsection{Problem 2}

Find the general solution of the differential equation. Then, use the initial condition to find the corresponding particular solution.
$$ xy' + 5y = 6x $$
First multiply each side by the integrating factor $ \frac{1}{x} $ to get the form $ y' + P(x)y = Q(x), y(3) = 6 $
\begin{align*}
    y' + \frac{5}{x}y & = 6 \\
                      & \therefore P(x) = \frac{5}{x}, \rho(x) = e^{\int(\frac{5}{x})dx} \\
    y(x) & = e^{-\int(\frac{5}{x})dx} \left[ \int \left( 6e^{\int(\frac{5}{x})dx} \right) dx + C \right]
         & = x^{-5} \left[ \int (6x^5)dx + C \right] \\
         & = x^{-5} \left[ x^6 + C \right] \\
         & = x + Cx^{-5} \\
    y(3) & = (3) + C(3)^{-5} = 6 \\
    \frac{1}{243}C & = 3 \\
    C & = 729
\end{align*}
\begin{equation*}
    \boxed{
        y(x) = x + Cx^{-5}, y(3) \rightarrow y(x) = x + 729x^{-5}
    }
\end{equation*}

\end{document}
