\documentclass{article}

% Document extensibility %
%
% Disables native paragraph indentation
\usepackage{parskip}
%
% Provides further bullet options for lists
\usepackage{enumitem}

% Mathematical symbol and statement packages %
%
% Necessary
\usepackage{amsmath}
\usepackage{amssymb}
%
% Extensive fraction notation
\usepackage{xfrac}
%
% Generic mathematical commands
% Notable: \degree, \celcius
\usepackage{gensymb}
%
% Variable vector notation (arrow above variable)
\usepackage{esvect}
%
% Multiline boxed equations
\usepackage{empheq}
%
% SI Unit
\usepackage{siunitx}
\usepackage{physunits}
%
% More intuitive arrays/matrices
\usepackage{array}
%
% Linear Equations
\usepackage{systeme}
%
% Boxes!
\usepackage{mdframed}
%
% Matrix Notation
\usepackage{bm}

% Graphic packages %
%
% Diagrams and illustrations
\usepackage{tikz}
\usetikzlibrary{positioning}
%
% Image insertion
\usepackage{graphicx}

% LaTeX Commands
%
% Argument Parser
\usepackage{xparse}

% Document content %
%
% Change title of table of contents
% \renewcommand{\contentsname}{Title}

\begin{document}

% Command `\hr` to insert horizontal rules
\newcommand{\hr}{\par\noindent\rule{\textwidth}{0.4pt}}

% Command to box and center math equations
\newcommand{\bc}[1]{
	\begin{equation*}
		\begin{boxed}
			{#1}
		\end{boxed}
	\end{equation*}
}

% Command for single line equations with a condition
\newcommand{\cond}[2]{
	\ifmmode
	{#1} \quad {#2}
	\else
	$$ {#1} \quad {#2} $$
	\fi
}

% Matrix and Vector notation
\newcommand{\matr}[1]{
	\ifmmode \bm{#1}
	\else \textit{\textbf{#1}}
	\fi
}
\newcommand{\vect}[1]{
	\ifmmode \mathbf{#1}
	\else \textbf{#1}
	\fi
}

% Laplace
\NewDocumentCommand{\lap}{o}{
	\IfNoValueTF{#1}
	{ \mathcal{L} }
	{ \mathcal{L} \left\{ {#1} \right\} }
}
\NewDocumentCommand{\ilap}{o}{
	\IfNoValueTF{#1}
	{ \mathcal{L}^{-1} }
	{ \mathcal{L}^{-1} \left\{ {#1} \right\} }
}

\tableofcontents

\section{Chapter 02 - Basic Structures}

\subsection{Sets}

\textbf{$ \in $}: belong to, is in

\subsubsection{Definition 2}

Two sets are equal if and only if they have the same elements. Therefore, if $ A $ and $ B $ are sets, then $ A $ and $ B $ are equal if and only if $ \forall x \left( x \in A \iff x \in B \right) $. We write $ A = B $ if $ A $ and $ B $ are equal sets.

\subsubsection{Definition 3}

The set $ A $ is also a subset of $ B $, and $ B $ is a superset of $ A $, if and only if every element of $ A $ is also an element of $ B $. We use the notation $ A \subseteq B $ to indicate that $ A $ is a subset of the set $ B $. If, instead, we want to stress that $ B $ is a superset of $ A $, we use the equivalent notation $ B \supseteq A $. (So, $ A \subseteq B $ and $ B \supseteq A $ are equivalent statements.)

\subsubsection{Definition 4}

Let $ S $ be a set. If there are exactly $ n $ distinct elements in $ S $ where $ n $ is a nonnegative integer, we say that $ S $ is a finite set and that $ n $ is the cardinality of $ S $. The cardinality of $ S $ is denoted by $ |S| $.

\subsubsection{Countable and Uncountable Sets}

\begin{itemize}
	\item Countable
	      \begin{itemize}
		      \item $ \mathbb{N} $
		      \item $ \mathbb{Z} $
		      \item $ \mathbb{Q} $
	      \end{itemize}
	\item Uncountable
	      \begin{itemize}
		      \item $ \mathbb{R} $
		      \item $ \mathbb{C} $
	      \end{itemize}
\end{itemize}

Let $ S_0 = \left\{ x \right\} $, and $ S_1 = \left\{ \left\{ x \right\} \right\} $.
\begin{equation}
	S_0 \neq S_1
\end{equation}

\subsubsection{Example}

\begin{enumerate}
	\item List the members of these sets.
	      \begin{enumerate}[label = \textbf{\alph*)}]
		      \item $ \left\{ x \mid x \text{ is a real number such that } x^2 = 1 \right\} $
		            \begin{align*}
			            S & = \left\{ x \in \mathbb{R} \mid x^2 = 1 \right\}
		            \end{align*}
		      \item $ \left\{ x \mid x \text{ is a positive integer less than 12} \right\} $
		            \begin{align*}
			            S & = \left\{ x \in \mathbb{R} \mid 0 \leq x < 12 \right\}
		            \end{align*}
	      \end{enumerate}
\end{enumerate}

\subsubsection{Definition 6}

Given a set $ S $, the power set of $ S $ is the set of all subsets of the set $ S $. The power set of $ S $ is denoted by $ \mathcal{P}(S) $.

\subsection{Set Operations}

\subsubsection{Definition 1}

Let $ A $ and $ B $ be sets. The union of the sets $ A $ and $ B $, denoted by $ A \cup B $, is the set that contains those elements that are either in $ A $ or in $ B $, or in both.
\begin{equation}
	A \cup B = \left\{ x \in U \mid ( x \in A ) \lor ( x \in B ) \right\}
\end{equation}

\subsubsection{Definition 2}

Let $ A $ and $ B $ be sets. The intersection of the sets $ A $ and $ B $, denoted by $ A \cap B $, is the set containing those elements in both $ A $ and $ B $.
\begin{equation}
	A \cap B = \left\{ x \in U \mid ( x \in A ) \land ( x \in B ) \right\}
\end{equation}

\subsubsection{Definition 3}

Two sets are disjoint if their intersection is the empty set.

\subsubsection{Definition 4}

Let $ A $ and $ B $ be sets. The difference of $ A $ and $ B $, denoted by $ A - B $, is the set containing those elements that are in $ A $ but not in $ B $. The difference of $ A $ and $ B $ is also called the complement of $ B $ with respect to $ A $.

\subsubsection{Definition 5}

Let $ U $ be the universal set. The complement of the set $ A $, denoted by $ \bar{A} $, is the complement of $ A $ with respect to $ U $. Therefore, the complement of the set $ A $ is $ U - A $.

\subsubsection{Proof}

Let $ A $, $ B $ be sets from $ U $. Show that $ A \subseteq B $ if and only if $ \overline{B} \subseteq \overline{A} $.

\textbf{Proof}:
\begin{itemize}
	\item For ``$ \implies $"

	      Given $ A \subseteq B $, need to show $ \overline{B} \subseteq \overline{A} $. Then $ \forall x \in A $, we have $ x \in B $.

	      By contrapositive we have
	      \begin{align*}
		      \neg \left( x \in B \right) & \implies \neg \left( x \in A \right)                           \\
		      x \notin B                  & \implies x \notin A, \quad \overline{B} \subseteq \overline{A} \\
	      \end{align*}
	\item For ``$ \impliedby $"

	      Given $ \overline{B} \subseteq \overline{A} $, we have $ \forall y \in \overline{B} $, $ y \in \overline{A} $ then the contrapositive is
	      \begin{align*}
		      \neg \left( y \in \overline{A} \right) & \implies \neg \left( y \in \overline{B} \right) \\
		      y \in A                                & \implies y \in B
	      \end{align*}
\end{itemize}

\subsubsection{Proof:}

Use the identities to show that $ \overline{ \left( A \cup B \right) } \cap \overline{ \left( B \cup C \right) } \cap \overline{ \left( A \cup C \right) } = \overline{A} \cap \overline{B} \cap \overline{C} $

\textbf{Proof}:
\begin{align*}
	\overline{A} \cap \overline{B} \cap \overline{C} & = \left( \overline{A} \cap \overline{B} \right) \cap \left( \overline{B} \cap \overline{C} \right) \cap \left( \overline{A} \cap \overline{C} \right) \\
	                                                 & = \overline{A} \cap \left( \overline{B} \cap \overline{B} \right) \cap \left( \overline{C} \cap \overline{C} \right) \cap \overline{A}                \\
	                                                 & = \overline{A} \cap \overline{B} \cap \overline{C}
\end{align*}

\subsubsection{Union}

The union is a collection of sets is the set that contains those elements that are member s of at least one set in the collection.

\begin{align*}
	A_1 \cup A_2 \cup \cdots \cup A_n & = \bigcup_{ i = 1 }^{ n } A_i
\end{align*}

\subsubsection{Intersection}

The intersection of a collection of sets is the set that contains those elements that are members of all the sets in the collection.

\begin{align*}
	A_1 \cap A_2 \cap \cdots \cap A_n & = \bigcap_{ i = 1 }^{ n } A_i
\end{align*}

\subsection{Functions}

\begin{itemize}
	\item Sets: $ A $, $ B $, $ C $, domain, codomain, range

	\item Relations: functions ($ f $, $ g $, $ h $)

	\item Elements: image, preimage
\end{itemize}

\subsubsection{Example}

\begin{align*}
	f_1 : \mathbb{R} \rightarrow \mathbb{R} \text{ as } y & = f_1(x) = 3x - 2 \\
	f_2 : \mathbb{R} \rightarrow \mathbb{R} \text{ as } y & = e^{x}           \\
	f_3 : \mathbb{R} \rightarrow \mathbb{R} \text{ as } y & = \sqrt{x}
\end{align*}
\begin{align*}
	f               & : A \rightarrow B                                           \\
	\text{range}(f) & = \left\{ y \in B \mid \forall x \in S \subseteq A \right\}
\end{align*}

\subsubsection{Properties}

\begin{enumerate}[label = \textbf{\arabic*)}]
	\item \label{function:property:1} $ f $ is injective – one-to-one \\
	\item \label{function:property:2} $ f $ is surjective – \\
	\item $ f $ is bijective if \ref{function:property:1} and \ref{function:property:2}
\end{enumerate}

Let $ f : A \rightarrow B $ be a function.

We say $ f $ is injective if
\begin{equation*}
	\left( x_1 \neq x_2 \implies f(x_1) \neq f(x_2) \right) \iff \left( f(x_1) = f(x_2) \implies x_1 = x_2 \right)
\end{equation*}
We say $ f $ is surjective if $ \forall y \in B $, $ \exists x \in A $ such that $ y = f(x) \iff \text{range}(f) = B $

We say $ f $ is bijective if $ f $ is injective and surjective.

\textbf{Monotonic Function}: We say $ f $ is increasing (strictly increasing) if $ x_1 > x_2 \implies f(x_1) > f(x_2) $

\subsubsection{Example 2.3.24}

Let $ f: \mathbb{R} \rightarrow \mathbb{R} $ and let $ f(x) > 0 $ for all $ x \in \mathbb{R} $. Show that $ f(x) $ is strictly increasing if and only if the function $ g(x) = \frac{ 1 }{ f(x) } $ is strictly decreasing.
\begin{align*}
	 & \rightarrow \frac{ 1 }{ f(x_1) } < \frac{ 1 }{ f(x_2) }                                                                       \\
	 & \rightarrow f(x_1) \cdot f(x_2) \left( \frac{ 1 }{ f(x_1) } \right) < f(x_1) \cdot f(x_2) \left( \frac{ 1 }{ f(x_2) } \right) \\
	 & \rightarrow f(x_2) < f(x_1)
\end{align*}
where the first implication comes from the fact that $ f(x) > 0, \forall x \in \mathbb{R} $.

\subsubsection{Example 2.3.73.b}

Prove or disprove each of these statements about the floor and ceiling functions.

\begin{equation*}
	\left\lfloor 2x \right\rfloor = 2 \left\lfloor x \right\rfloor
\end{equation*}

Consider $ x = 1.6 $
\begin{align*}
	\left\lfloor 2x \right\rfloor  & = \left\lfloor 2 \cdot 1.6 \right\rfloor = \left\lfloor 3.2 \right\rfloor = 3 \\
	2 \left\lfloor x \right\rfloor & = 2 \left\lfloor 1.6 \right\rfloor = 2(1) = 2
\end{align*}
Hence $ \left\lfloor 2x \right\rfloor = 2 \left\lfloor x \right\rfloor $ for all $ x \in \mathbb{R} $ is false.

\subsubsection{Inverse Function}

Let $ f: A \rightarrow B $ be a function. If $ f $ is injective, then there exists $ g: B \rightarrow A $ such that $ f \cdot g \left( y \right) = y, \forall y \in B $ and $ g \cdot f \left( x \right) = x, \forall x \in A $. We call $ g $ the inverse of $ f $. We can denote $ g = f^{-1} $.

\subsection{Sequences and Summations}

Let $ f: A \rightarrow B $ where $ A = \left\{ 1, 2, 3, \cdots \right\} $ or $ \left\{ 0, 1, 2, 3, \cdots \right\} $, $ B = \mathbb{R} $.

Special sequences:
\begin{itemize}
	\item Geometric Sequence
	      \begin{equation}
		      a_n = a_1r^{n - 1} = a_0r^{n}
	      \end{equation}
	\item Arithmetic Sequence
	      \begin{equation}
		      a_n = a_1 + (n - 1)d = a_0 + nd
	      \end{equation}
	\item Fibonacci Sequence: $ f_0, f_1, f_2, \cdots $ is defined by the initial conditions $ f_0 = 0, f_1 = 1 $ and the recurrence relation
	      \begin{equation}
		      f_n = f_{n - 1} + f_{n - 2}
	      \end{equation}
\end{itemize}

In order to describe a sequence:
\begin{itemize}
	\item Closed formula
	\item Recurrence relation
	\item Verbally
\end{itemize}

\subsubsection{Geometric Sequence}

If $ r = 1 $ then $ a_n = ar^{n} = a $ then $ \sum_{j = 0}^{n} ar^{j} = \sum_{j = 0}^{n} a = (n - 0 + 1)a $.

Let $ k = j + 1 $.
\begin{align*}
	j & = k - 1                                    \\
	j & = 0, k = 1                                 \\
	  & = \sum_{j = 0}^{j = n} ar^{j + 1}          \\
	  & = \sum_{k = 1}^{k = n + 1} ar^{k}          \\
	  & = a + ar + ar^2 + \cdots + ar^{n + 1} - a  \\
	  & = \sum_{k = 0}^{n} ar^{k} + ar^{n + 1} - a
\end{align*}

If $ r \neq 1 $

Notice that $ \left( 1 - x \right) \left( 1 + x + x^2 + \cdots + x^{n} \right) = 1+ (x - x) + (x^2 - x^2) + \cdots + (x^{n} - x^{n}) - x^{n + 1} = 1 - x^{n + 1} $

Then
\begin{align*}
	\sum_{j = 0}^{n} ar^{j} & = a + ar + ar^2 + \cdots + ar^{n}                  \\
	                        & = a \left( 1 + r + r^2 + \cdots + r^{n} \right)    \\
	                        & = a \left( \frac{ 1 - r^{n + 1} }{ 1 - r } \right) \\
	                        & = a \left( \frac{ r^{n + 1} - 1 }{ r - 1 } \right)
\end{align*}

\subsubsection{Practice}

Prove $ \sum_{k = 1}^{n} k = 1 + 2 + 3 + \cdots + k = \frac{ n(n + 1) }{ 2 } $
\begin{enumerate}[label = \textbf{Method \arabic*:}]
	\item
	      \begin{align*}
		      \sum_{k = 1}^{n} k         & = 1 + 2 + 3 + \cdots + n                                                                                                     \\
		      2 \cdot \sum_{k = 1}^{n} k & = \left( 1 + 2 + 3 + \cdots + n \right) + \left( 1 + 2 + 3 + \cdots + n \right)                                              \\
		                                 & = \sum_{k = 1}^{n} \left( n + 1 \right) = \left( n + 1 \right) \cdot \left( n - 1 + n \right) = \left( n + 1 \right) \cdot n \\
		      \sum_{k = 1}^{n} k         & = \frac{ n \left( n + 1 \right) }{ 2 }
	      \end{align*}

	\item Telescoping

	      Notice that
	      \begin{align*}
		      \sum_{k = 0}^{n - 1} \left( a_{k + 1} - a_{k} \right)        & = a_1 - a_0 + a_2 - a_1 + a_3 - a_2 + \cdots + a_{n} - a_{n - 1}                              \\
		                                                                   & = \sum_{i = 1}^{n} \left( a_{i} - a_{i - 1} \right) = a_n - a_0                               \\
		      \text{and, } i^2 - \left( i - 1 \right)^{2}                  & = i^2 - \left( i^2 - 2i + 1 \right) = 2i - 1                                                  \\
		      \sum_{i = 1}^{n} \left( i^2 - \left( i - 1 \right)^2 \right) & = \sum_{i = 1}^{n} 2i - 1                                                                     \\
		      n^2 - 0^2                                                    & = 2 \sum_{i = 1}^{n} i - \sum_{i = 1}^{n} 1, \quad \text{where $ a_i = i^2 $ for telescoping} \\
		      \sum_{i = 1}^{n}                                             & = \frac{ n^2 + n }{ 2 }
	      \end{align*}
\end{enumerate}

Prove $ \sum_{k = 1}^{n} k^2 = 1^2 + 2^2 + 3^2 + \cdots + k^2 = \frac{ n \left( n + 1 \right) \left( 2n + 1 \right) }{ 6 } $, Let $ a_i = i^3 $
\begin{align*}
	\sum_{i = 1}^{n} \left( a_{i} - a_{i - 1} \right) & = a_{n} - a_0                                                                     \\
	i^3 - (i - 1)^{3}                                 & = 3i^2 - 3i + 1                                                                   \\
	\sum_{i = 1}^{n} \left( i^3 \right)               & = 3 \sum_{i = 1}^{n} i^2 - 3 \sum_{i = 1}^{n} i + \sum_{i = 1}^{n} 1              \\
	3 \sum_{i = 1}^{n} i^2                            & = \sum_{i = 1}^{n} \left( i^3 \right) + 3 \sum_{i = 1}^{n} i - \sum_{i = 1}^{n} 1
\end{align*}

\subsection{Cardinality of Sets}

Compare numbers (including $ \infty $)

\begin{enumerate}
	\item Finite Elements
	      \begin{itemize}
		      \item Finite: $ 0, 1, 2, 3, \cdots, n $
	      \end{itemize}

	\item Infinitely Many Elements
	      \begin{itemize}
		      \item Countable: $ \mathbb{N} = \mathbb{Z}^{+}, \mathbb{Z}, \mathbb{Q} $

		            For $ \mathbb{Z} $:
		            \begin{tabular}{ | c | c | }
			            $ \mathbb{N} $ & $ \mathbb{Z}^{+} $ \\
			            \hline
			            1              & 0                  \\
			            2              & 1                  \\
			            3              & -1                 \\
			            4              & 2                  \\
			            5              & -2                 \\
			            6              & 3                  \\
			            7              & -3
		            \end{tabular}

		            For $ \mathbb{Q} = \left\{ \frac{ m }{ n } \mid m \in \mathbb{Z}, n \in \mathbb{Z}^{+}, n \neq 0, \text{gcd}\left( m, n \right) = 1 \right\} $

		      \item Uncountable: $ \mathbb{R}, \mathbb{R}^2, \cdots, \mathbb{R}^{n} $
	      \end{itemize}
\end{enumerate}

\subsubsection{Shroder-Bernstein Theorem Example}

Let $ A = [0, 1], B = (0, 1) $. Show that $ |A| = |B| $.

\textbf{Proof}:
\begin{itemize}
	\item Consider $ f_1: B \rightarrow A \text{ as } f(x) = x $. Thus $ f_1 $ is one-to-one $ \implies |B| \leq |A| $.

	\item Next consider $ f_2: A \rightarrow B \text{ as } f(x) = \frac{ x }{ 2 } + a, x \in \left[ 0, 1 \right], a \in \left( 0, \frac{ 1 }{ 2 } \right) $. Then $ f(A) = \left[ a, \frac{ 1 }{ 2 } + a \right] \subseteq B $. Thus $ f_2 $ is one-to-one $ \implies |A| \leq |B| $.
\end{itemize}

\subsection{Matrices}

\end{document}
