\documentclass{article}

% Document extensibility %
%
% Disables native paragraph indentation
\usepackage{parskip} 
%
% Provides further bullet options for lists
\usepackage{enumitem}

% Mathematical symbol and statement packages %
%
% Necessary
\usepackage{amsmath}
\usepackage{amssymb}
%
% Extensive fraction notation
\usepackage{xfrac}
%
% Generic mathematical commands
% Notable: \degree, \celcius
\usepackage{gensymb}
%
% Variable vector notation (arrow above variable)
\usepackage{esvect}
%
% Multiline boxed equations
\usepackage{empheq}
%
% SI Unit
\usepackage{siunitx}

% Graphic packages %
%
% Diagrams and illustrations
\usepackage{tikz}
%
% Image insertion
\usepackage{graphicx}

% Document content %
%
% Change title of table of contents
% \renewcommand{\contentsname}{Title}

\begin{document}

% Command `\hr` to insert horizontal rules
\newcommand{\hr}{\par\noindent\rule{\textwidth}{0.4pt}}

% Command to box and center math equations
\newcommand{\bc}[1]{
	\begin{equation*}
		\begin{boxed}
			{#1}
		\end{boxed}
	\end{equation*}
}

% Command for single line equations with a condition
\newcommand{\cond}[2]{
	\ifmmode
		{#1} \quad {#2}
	\else
		$$ {#1} \quad {#2} $$
	\fi
}

\tableofcontents

\section{Section 5.5}

\subsection{5.5.2}
Find a particular solution $ y_p $ of the following equation using the Method of Undetermined Coefficients. Primes denote the derivatives with respect to $ x $.
$$ y'' - y' - 2y = 4x + 6 $$
\begin{align*}
	r^2 - r - 2 & = 0 \\
	r & = 2, -1 \\
	y(x) & = c_1e^{2x} + c_2e^{-x} \\
	y_p(x) & = Ax + B \\
	y_p'(x) & = A \\
	y_p''(x) & = 0
\end{align*}
\begin{align*}
	(0) - (A) - 2(Ax + B) & = 4x + 6 \\
	-2Ax - A - 2B & = 4x + 6 \\
	-2A & = 4 \\
	A & = -2 \\
	-A - 2B & = 6 \\
	-(-2) - 2B & = 6 \\
	B & = -2 \\
	y(x) & = -2x - 2
\end{align*}
\bc{y(x) = -2x - 2}

\subsection{5.5.3}
Find a particular solution $ y_p $ of the following equation using the Method of Undetermined Coefficients. Primes denote the derivatives with respect to $ x $.
$$ y'' - y' - 6y = 20\sin(3x) $$
\begin{align*}
	r^2 - r - 6 & = 0 \\
	r & = 3, -2 \\
	y(x) & = c_1e^{3x} + c_2e^{-2x} \\
	y_p(x) & = A\cos(3x) + B\sin(3x) \\
	y_p'(x) & = -3A\sin(3x) + 3B\cos(3x) \\
	y_p''(x) & = -9A\cos(3x) + -9B\sin(3x) \\
	20\sin(3x) & = (-9A\cos(3x) + -9B\sin(3x)) - (-3A\sin(3x) + 3B\cos(3x)) - 6(A\cos(3x) + B\sin(3x))
\end{align*}
\begin{align*}
	\cos(3x)(-9A - 3B - 6A) + \sin(3x)(-9B + 3A - 6B) & = 20\sin(3x) \\
	-9A - 3B - 6A & = 0 \\
	-15A - 3B & = 0 \\
	B & = -5A \\
	-9B + 3A - 6B & = 20 \\
	-15B + 3A & = 20 \\
	-15(-5A) + 3A & = 20 \\
	A & = \frac{10}{39} \\
	B & = -5 \left( \frac{10}{39} \right) \\
	B & = -\frac{50}{39} \\
	y(x) & = \frac{10}{39}\cos(3x) - \frac{50}{39}\sin(3x)
\end{align*}
\bc{y(x) = \frac{10}{39}\cos(3x) - \frac{50}{39}\sin(3x)}

\subsection{5.5.4}
Find a particular solution $ y_p $ of the following equation using the Method of Undetermined Coefficients. Primes denote the derivatives with respect to $ x $.
$$ y'' - 4y' + 5y = xe^x $$
\begin{align*}
	r^2 - 4r + 5 & = 0 \\
	r & = 2 \pm 1i \\
	y(x) & = c_1e^{2x}\cos(x) + c_2e^{2x}\sin(x) \\
	y_p(x) & = (Ax + B)Ce^x \\
	y_p(x) & = e^x(Ax + B) \\
	y_p'(x) & = e^x(Ax + A + B) \\
	y_p''(x) & = e^x(Ax + 2A + B) \\
	xe^x & = (e^x(Ax + 2A + B)) - 4(e^x(Ax + A + B)) + 5(e^x(Ax + B))
\end{align*}
\begin{align*}
	xe^x(A - 4A + 5A) + e^x(2A + B - 4A - 4B + 5B) & = xe^x \\
	A - 4A + 5A & = 1 \\
	A & = \frac{1}{2} \\
	2A + B - 4A - 4B + 5B & = 0 \\
	-2A + 2B & = 0 \\
	-2 \left( \frac{1}{2} \right) + 2B & = 0 \\
	B & = \frac{1}{2} \\
	y(x) & = e^x \left( \frac{x}{2} + \frac{1}{2} \right)
\end{align*}
\bc{y(x) = e^x \left( \frac{x}{2} + \frac{1}{2} \right)}

\subsection{5.5.10}
Find a particular solution $ y_p $ of the following equation using the Method of Undetermined Coefficients. Primes denote the derivatives with respect to $ x $.
$$ y'' + 9y = 4\cos(3x) + 6\sin(3x) $$
\begin{align*}
	r^2 + 9 & = 0 \\
	r & = 0 \pm 3i \\
	y(x) & = c_1\cos(3x) + c_2\sin(3x) \\
	y_p(x) & = A\cos(3x) + B\sin(3x) \\
	y_p'(x) & = -3A\sin(3x) + 3B\cos(3x) \\
	y_p''(x) & = -9A\cos(3x) - 9B\sin(3x) \\
			 & (-9A\cos(3x) - 9B\sin(3x)) + 9(A\cos(3x) + B\sin(3x)) \\
			 & = 4\cos(3x) + 6\sin(3x)
\end{align*}
\begin{align*}
	\cos(3x)(-9A + 9A) + \sin(3x)(-9B + 9B) & = 4\cos(3x) + 6\sin(3x)
\end{align*}

\end{document}
