\documentclass{article}

% Document extensibility %
%
% Disables native paragraph indentation
\usepackage{parskip} 
%
% Provides further bullet options for lists
\usepackage{enumitem}

% Mathematical symbol and statement packages %
%
% Necessary
\usepackage{amsmath}
\usepackage{amssymb}
%
% Extensive fraction notation
\usepackage{xfrac}
%
% Generic mathematical commands
% Notable: \degree, \celcius
\usepackage{gensymb}
%
% Variable vector notation (arrow above variable)
\usepackage{esvect}
%
% Multiline boxed equations
\usepackage{empheq}
%
% SI Unit
\usepackage{siunitx}
\usepackage{physunits}
%
% More intuitive arrays/matrices
\usepackage{array}
%
% Linear Equations
\usepackage{systeme}
%
% Boxes!
\usepackage{mdframed}
%
% Matrix Notation
\usepackage{bm}

% Graphic packages %
%
% Diagrams and illustrations
\usepackage{tikz}
\usetikzlibrary{positioning}
%
% Image insertion
\usepackage{graphicx}

% Document content %
%
% Change title of table of contents
% \renewcommand{\contentsname}{Title}

\begin{document}

% Command `\hr` to insert horizontal rules
\newcommand{\hr}{\par\noindent\rule{\textwidth}{0.4pt}}

% Command to box and center math equations
\newcommand{\bc}[1]{
	\begin{equation*}
		\begin{boxed}
			{#1}
		\end{boxed}
	\end{equation*}
}

% Command for single line equations with a condition
\newcommand{\cond}[2]{
	\ifmmode
		{#1} \quad {#2}
	\else
		$$ {#1} \quad {#2} $$
	\fi
}

% Matrix and Vector notation
\newcommand{\matr}[1]{
	\ifmmode \bm{#1}
	\else \textit{\textbf{#1}}
	\fi
}
\newcommand{\vect}[1]{
	\ifmmode \mathbf{#1}
	\else \textbf{#1}
	\fi
}

% Laplace
\newcommand{\lap}{\mathcal{L}}
\newcommand{\ilap}{\mathcal{L}^{-1}}

\tableofcontents

\section{Part 1}

Take the Laplace Transformation of the following initial valued problem and solve for $ Y(s) $:

\begin{enumerate}[label = \textbf{\arabic*)}]
	\item
		\begin{equation*}
			y'' + 5y' + 6y = 12e^t, y(0) = -1, y'(0) = 7
		\end{equation*}
		\begin{align*}
			\lap(y'') + 5\lap(y') + 6\lap(y) & = 12\lap(e^t) \\
			\left[ s^2\lap(y) - sy(0) - y'(0) \right] + 5 \left[ s\lap(y) - y(0) \right] + 6\lap(y) & = \frac{12}{s - 1} \\
			\lap(y)(s^2 + 5s + 6) + s - 7 + 5 & = \frac{12}{s - 1} \\
			\lap(y) & = \frac{-s^2 + 3s + 10}{(s - 1)(s^2 + 5s + 6)} \\
			\lap(y) & = -\frac{s - 5}{(s - 1)(s + 3)} \\
			\lap(y) & = -\frac{1}{s - 1} + \frac{2}{s + 3}
		\end{align*}
		\begin{align*}
			y & = -\ilap \left( \frac{1}{s - 1} \right) + 2\ilap \left( \frac{1}{s + 3} \right) \\
			y & = e^t - 2e^{-3t}
		\end{align*}
		\bc{ y = e^t - 2e^{-3t} }
	\item
		\begin{equation*}
			y'' - 7y' + 10y = 9\cos(t) + 7\sin(t), y(0) = 5, y'(0) = -4
		\end{equation*}
		\begin{align*}
			\lap(y'') - 7\lap(y') + 10\lap(y) & = 9\lap(\cos(t)) + 7\lap(\sin(t)) \\
			\left[ s^2\lap(y) - sy(0) - y'(0) \right] - 7 \left[ s\lap(y) - y(0) \right] + 10\lap(y) & = \frac{9s}{s^2 + 1} + \frac{7}{s^2 + 1} \\
			\lap(y)(s^2 - 7s + 10) - 5s + 4 + 35 & = \frac{9s + 7}{s^2 + 1} \\
			\lap(y) & = \frac{5s^3 - 39s^2 + 14s - 32}{(s^2 + 1)(s^2 - 7s + 10)} \\
			\lap(y) & = \frac{s}{s^2 + 1} + \frac{8}{s - 2} - \frac{4}{s - 5}
		\end{align*}
		\begin{align*}
			y & = \ilap \left( \frac{s}{s^2 + 1} \right) + 8\ilap \left( \frac{1}{s - 2} \right) - 4\ilap \left( \frac{1}{s - 5} \right) \\
			y & = \cos(t) + 8e^{2t} - 4e^{5t}
		\end{align*}
		\bc{ y = \cos(t) + 8e^{2t} - 4e^{5t} }
	\item
		\begin{equation*}
			y'' - 4y = 4t - 8e^{-2t}, y(0) = 0, y'(0) = 5
		\end{equation*}
		\begin{align*}
			\lap(y'') - 4\lap(y) & = 4\lap(t) - 8\lap(e^{-2t}) \\
			\left[ s^2\lap(y) - sy(0) - y'(0) \right] - 4\lap(y) & = \frac{4}{s^2} - \frac{8}{s + 2} \\
			\lap(y)(s^2 - 4) - 0 - 5 & = \frac{4}{s^2} - \frac{8}{s + 2} \\
			\lap(y) & = \frac{5s^3 + 2s^2 + 4s + 8}{s^2(s + 2)(s^2 - 4)} \\
			\lap(y) & = -\frac{1}{s^2} - \frac{1}{s + 2} + 2\frac{1}{(s + 2)^2} + \frac{1}{s - 2}
		\end{align*}
		\begin{align*}
			y & = -\ilap \left( \frac{1}{s^2} \right) - \ilap \left( \frac{1}{s + 2} \right) + 2\ilap \left( \frac{1}{(s + 2)^2} \right) + \ilap \left( \frac{1}{s - 2} \right) \\
			y & = -t - e^{-2t} + 2te^{-2t} + e^{2t}
		\end{align*}
		\bc{ y = -t - e^{-2t} + 2te^{-2t} + e^{2t} }
\end{enumerate}

\end{document}
